### Proof Using Mathematical Induction

We are tasked with proving the following equation for all non-negative integers \( n \):

\[
2^0 + 2^1 + \cdots + 2^n = 2^{n+1} - 1
\]

#### Base Case:
Let \( n = 0 \). Then, the left-hand side of the equation is:

\[
2^0 = 1
\]

The right-hand side is:

\[
2^{0+1} - 1 = 2^1 - 1 = 1
\]

Since both sides are equal, the equation holds for \( n = 0 \). This satisfies the base case as required.

#### Inductive Step:
Now, let \( n \) be an arbitrary natural number. Assume that the statement holds true for \( n \), i.e.,

\[
2^0 + 2^1 + \cdots + 2^n = 2^{n+1} - 1
\]

We need to prove that the equation also holds for \( n + 1 \). Consider the sum up to \( n + 1 \):

\[
2^0 + 2^1 + \cdots + 2^{n+1}
\]

Using the inductive hypothesis, we can substitute the sum up to \( n \) as follows:

\[
(2^0 + 2^1 + \cdots + 2^n) + 2^{n+1} = (2^{n+1} - 1) + 2^{n+1}
\]

Simplifying the right-hand side:

\[
(2^{n+1} - 1) + 2^{n+1} = 2 \cdot 2^{n+1} - 1 = 2^{n+2} - 1
\]

Thus, the equation holds for \( n + 1 \).

By the principle of mathematical induction, we have proven that:

\[
2^0 + 2^1 + \cdots + 2^n = 2^{n+1} - 1
\]

for all \( n \geq 0 \), completing the proof.
