**Note for Question Lab 2, Number 5**

## Proof Using Mathematical Induction

We are tasked with proving the equation:

\[
2^0 + 2^1 + \cdots + 2^n = 2^{n+1} - 1
\]

### Base Case:
Let \( n = 0 \). Then we have:

\[
2^0 = 1 = 2^{1} - 1
\]

This satisfies the equation as required.

### Induction Step:
Now, let \( n \) be an arbitrary natural number. Assume the statement holds true for \( n \), i.e.,

\[
2^0 + 2^1 + \cdots + 2^n = 2^{n+1} - 1
\]

We need to prove that it holds for \( n + 1 \). Consider:

\[
2^0 + 2^1 + \cdots + 2^{n+1}
\]

Using the inductive hypothesis, we can rewrite this as:

\[
(2^0 + 2^1 + \cdots + 2^n) + 2^{n+1} = (2^{n+1} - 1) + 2^{n+1}
\]

Simplifying the right-hand side:

\[
= 2 \cdot 2^{n+1} - 1 = 2^{n+2} - 1
\]

Thus, the statement holds for \( n + 1 \), completing the proof.
